fix(KSA-Dafny): break up Mutations, other fixes, more tests (#1069)
Fixes:
- Wrong assertion for Java Example Test of In-Flight Mutation scanner
- Initialize Mutation, when using Decrypt/Encrypt, must use Decrypt/Encrypt to mutate the Beacon

Tests:
- Explicitly Test Decrypt/Encrypt with different credentials that only can use the relevant KMS Keys
- Refactor Examples to be easier to test across inputs

Other:
- Add Documentation to the Java Examples

Co-authored-by: José Corella <39066999+josecorella@users.noreply.github.com>

AwsCryptographicMaterialProviders/dafny/AwsCryptographyKeyStore/src/Structure.dfy
@@ -146,6 +146,16 @@ module {:options "/functionSyntax:4" } Structure {
        )
   }
 
+  predicate ActiveHierarchicalSymmetricVersionEncryptionContext?(
+    ec: Types.EncryptionContextString
+  )
+  {
+    && BranchKeyContext?(ec)
+    && BRANCH_KEY_ACTIVE_VERSION_FIELD in ec
+    && ec[TYPE_FIELD] == BRANCH_KEY_ACTIVE_TYPE
+  }
+
+
   function ToAttributeMap(
     key: Types.EncryptedHierarchicalKey
   ): (output: DDB.AttributeMap)
